examples/low-level/crypto/Crypto.Symmetric.Poly1305_64.Spec.fst
@@ -1,0 +1,244 @@
+module Crypto.Symmetric.Poly1305_64.Spec
+
+(* Just the mathematical specification,
+   used in the probabilistic security assumption,
+   aiming for a generic group *)
+
+open FStar.Mul
+open FStar.Ghost
+open FStar.Seq
+
+(** Machine integers *)
+open FStar.UInt8
+open FStar.UInt64
+open FStar.Int.Cast
+
+(** Mathematical definitions *)
+open FStar.Math.Lib
+open FStar.Math.Lemmas
+open Crypto.Symmetric.Bytes 
+
+module U8  = FStar.UInt8
+module U32 = FStar.UInt32
+module U64 = FStar.UInt64
+module H8   = Hacl.UInt8
+module H64  = Hacl.UInt64
+module H128 = Hacl.UInt128
+
+#reset-options "--initial_fuel 4 --max_fuel 4"
+
+let byte = if Flag.mac_log then U8.t else H8.t
+
+// prime (do we prove it? use it?)
+let p_1305: p:nat{pow2 128 < p} =
+  assert_norm (pow2 128 < pow2 130 - 5);
+  pow2 130 - 5
+
+#reset-options
+
+type elem = n:nat{n < p_1305} // elements of the field Z / p_1305 Z
+
+type word = b:seq byte {Seq.length b <= 16}
+type word_16 = b:seq byte {Seq.length b = 16}
+// we only use full words for AEAD
+
+type text = seq elem // not word_16
+type tag = word_16
+let taglen 'id = 16ul
+
+(* * *********************************************)
+(* *            Field operations                 *)
+(* * *********************************************)
+val field_add: elem -> elem -> Tot elem
+let field_add a b = (a + b) % p_1305
+val field_mul: elem -> elem -> Tot elem
+let field_mul a b = (a * b) % p_1305
+
+(* Infix field operators for readability *)
+let op_Plus_At = field_add
+let op_Star_At = field_mul
+
+
+
+
+(* REST OF THE FILE TO BE RESHUFFLED OR DELETED,
+   PARTLY COPIED TO BUFFER.UTIL OR ENCODING *)
+
+(* * *********************************************)
+(* *            Encoding                         *)
+(* * *********************************************)
+
+let encode (w:word) : Tot elem =
+  let l = length w in
+  pow2_le_compat 128 (8 * l);
+  pow2 (8 * l) +@ little_endian w
+
+// a spec for encoding and padding, convenient for injectivity proof
+// TODO: Unused now
+let pad_0 b l = Seq.append b (Seq.create l 0uy)
+
+val encode_pad: prefix:Seq.seq elem -> txt:Seq.seq UInt8.t -> GTot (Seq.seq elem) 
+  (decreases (Seq.length txt))
+let rec encode_pad prefix txt =
+  let l = Seq.length txt in
+  if l = 0 then prefix
+  else if l < 16 then
+    let w = txt in
+    SeqProperties.snoc prefix (encode w)
+  else
+    begin
+    let w, txt = SeqProperties.split txt 16 in
+    let prefix = SeqProperties.snoc prefix (encode w) in
+    encode_pad prefix txt
+    end
+
+
+let trunc_1305 (e:elem) : Tot elem = e % pow2 128
+
+(* * *********************************************)
+(* *          Encoding-related lemmas            *)
+(* * *********************************************)
+
+#reset-options "--initial_fuel 1 --max_fuel 1 --initial_ifuel 0 --max_ifuel 0"
+
+
+val lemma_pad_0_injective: b0:Seq.seq UInt8.t -> b1:Seq.seq UInt8.t -> l:nat -> Lemma
+  (requires (pad_0 b0 l == pad_0 b1 l))
+  (ensures  (b0 == b1))
+let lemma_pad_0_injective b0 b1 l =
+  SeqProperties.lemma_append_inj b0 (Seq.create l 0uy) b1 (Seq.create l 0uy);
+  Seq.lemma_eq_intro b0 b1
+
+val lemma_encode_injective: w0:word -> w1:word -> Lemma
+  (requires (length w0 == length w1 /\ encode w0 == encode w1))
+  (ensures  (w0 == w1))
+let lemma_encode_injective w0 w1 =
+  let l = length w0 in
+  lemma_little_endian_is_bounded w0;
+  lemma_little_endian_is_bounded w1;
+  pow2_le_compat 128 (8 * l);
+  lemma_mod_plus_injective p_1305 (pow2 (8 * l))
+    (little_endian w0) (little_endian w1);
+  assert (little_endian w0 == little_endian w1);
+  Seq.lemma_eq_intro (Seq.slice w0 0 l) w0;
+  Seq.lemma_eq_intro (Seq.slice w1 0 l) w1;
+  lemma_little_endian_is_injective w0 w1 l
+
+val lemma_encode_pad_injective: p0:Seq.seq elem -> t0:Seq.seq UInt8.t -> p1:Seq.seq elem -> t1:Seq.seq UInt8.t -> Lemma
+  (requires length t0 == length t1 /\ encode_pad p0 t0 == encode_pad p1 t1)
+  (ensures  p0 == p1 /\ t0 == t1)
+  (decreases (Seq.length t0))
+let rec lemma_encode_pad_injective p0 t0 p1 t1 =
+  let l = Seq.length t0 in
+  if l = 0 then Seq.lemma_eq_intro t0 t1
+  else if l < 16 then
+    begin
+    SeqProperties.lemma_append_inj
+      p0 (Seq.create 1 (encode t0))
+      p1 (Seq.create 1 (encode t1));
+    lemma_index_create 1 (encode t0) 0;
+    lemma_index_create 1 (encode t1) 0;
+    lemma_encode_injective t0 t1
+    end
+  else
+    begin
+    let w0, t0' = SeqProperties.split_eq t0 16 in
+    let w1, t1' = SeqProperties.split_eq t1 16 in
+    let p0' = SeqProperties.snoc p0 (encode w0) in
+    let p1' = SeqProperties.snoc p1 (encode w1) in
+    assert (encode_pad p0' t0' == encode_pad p1' t1');
+    lemma_encode_pad_injective p0' t0' p1' t1';
+    SeqProperties.lemma_append_inj
+      p0 (Seq.create 1 (encode w0))
+      p1 (Seq.create 1 (encode w1));
+    lemma_index_create 1 (encode w0) 0;
+    lemma_index_create 1 (encode w1) 0;
+    lemma_encode_injective w0 w1
+    end
+
+val encode_pad_empty: prefix:Seq.seq elem -> txt:Seq.seq UInt8.t -> Lemma
+  (requires Seq.length txt == 0)
+  (ensures  encode_pad prefix txt == prefix)
+let encode_pad_empty prefix txt = ()
+
+val encode_pad_snoc: prefix:Seq.seq elem -> txt:Seq.seq UInt8.t -> w:word_16 -> Lemma
+  (encode_pad (SeqProperties.snoc prefix (encode w)) txt ==
+   encode_pad prefix (append w txt))
+let encode_pad_snoc prefix txt w =
+  Seq.lemma_len_append w txt;
+  assert (16 <= Seq.length (append w txt));
+  let w', txt' = SeqProperties.split (append w txt) 16 in
+  let prefix' = SeqProperties.snoc prefix (encode w') in
+  Seq.lemma_eq_intro w w';
+  Seq.lemma_eq_intro txt txt'
+
+(* * *********************************************)
+(* *        Poly1305 functional invariant        *)
+(* * *********************************************)
+
+let seq_head (vs:seq 'a {Seq.length vs > 0}) = Seq.slice vs 0 (Seq.length vs - 1)
+
+val poly: vs:seq elem -> r:elem -> Tot (a:elem) (decreases (Seq.length vs))
+let rec poly vs r =
+  if Seq.length vs = 0 then 0
+  else (poly (seq_head vs) r +@ Seq.index vs (length vs - 1)) *@ r
+
+(* the definition above captures what POLY1305 does, 
+   not the usual polynomial computation; 
+   it may be more natural to flip the sequence, 
+   so that the coefficients are aligned. 
+   (i.e. a_0::a_1::a_2 stands for a_0 + a_1 X + a_2 X^2 , is implicitly extended with 0s.) *)
+
+val poly': vs:seq elem -> r:elem -> Tot (a:elem) (decreases (Seq.length vs))
+let rec poly' vs r =
+  if Seq.length vs = 0 then 0
+  else (SeqProperties.head vs +@ poly' (SeqProperties.tail vs) r ) *@ r
+
+val eq_poly0: p:seq elem -> Tot bool (decreases (length p)) 
+let rec eq_poly0 p = 
+  Seq.length p = 0 || 
+  (SeqProperties.head p = 0 && eq_poly0 (SeqProperties.tail p))
+  
+val eq_poly: p0:seq elem -> p1:seq elem -> Tot bool (decreases (length p0))
+let rec eq_poly p0 p1 = 
+  if Seq.length p0 = 0 then eq_poly0 p1 
+  else if Seq.length p1 = 0 then eq_poly0 p0
+  else SeqProperties.head p0 = SeqProperties.head p1 && eq_poly (SeqProperties.tail p0) (SeqProperties.tail p1)
+
+#set-options "--lax"
+private let rec lemma_sane_eq_poly0 (p:seq elem) (r:elem) : Lemma
+  (requires eq_poly0 p)
+  (ensures (poly' p r = 0)) (decreases (Seq.length p)) = 
+  if Seq.length p = 0 then () 
+  else if SeqProperties.head p = 0 then lemma_sane_eq_poly0 (SeqProperties.tail p) r
+#reset-options "--z3timeout 1000"
+private let rec lemma_sane_eq_poly (p0:seq elem) (p1:seq elem) (r:elem) : Lemma
+  (requires eq_poly p0 p1)
+  (ensures (poly' p0 r = poly' p1 r)) (decreases (Seq.length p0)) = 
+  if Seq.length p0 = 0 then lemma_sane_eq_poly0 p1 r 
+  else if Seq.length p1 = 0 then lemma_sane_eq_poly0 p0 r
+  else lemma_sane_eq_poly (SeqProperties.tail p0) (SeqProperties.tail p1) r
+
+
+//16-10-15 to stay close to the paper, we may apply "encode" in the poly specification
+
+private let fix (r:word_16) (i:nat {i < 16}) m : Tot word_16 =
+  Seq.upd r i (U8 (Seq.index r i &^ m))
+
+// an abstract spec of clamping for our state invariant
+// for our polynomial-sampling assumption,
+// we rely solely on the number of fixed bits (22, right?)
+val clamp: word_16 -> Tot elem
+let clamp r =
+  let r = fix r  3  15uy in // 0000****
+  let r = fix r  7  15uy in
+  let r = fix r 11  15uy in
+  let r = fix r 15  15uy in
+  let r = fix r  4 252uy in // ******00
+  let r = fix r  8 252uy in
+  let r = fix r 12 252uy in
+  little_endian r
+
+(** REMARK: this is equivalent to (poly vs r + little_endian s) % pow2 128 *)
+val mac_1305: vs:seq elem -> r:elem -> s:seq byte -> Tot int
+let mac_1305 vs r s = (trunc_1305 (poly vs r) + little_endian s) % pow2 128
