examples/low-level/crypto/Crypto.Symmetric.Poly1305_64.fst
@@ -1,0 +1,474 @@
+(* Implementation of Poly1305 based on the rfc7539 *)
+module Crypto.Symmetric.Poly1305_64
+
+open FStar.Mul
+open FStar.Ghost
+open FStar.Seq
+(** Machine integers *)
+open FStar.UInt8
+open FStar.UInt64
+open FStar.Int.Cast
+(** Effects and memory layout *)
+open FStar.HyperStack
+(** Buffers *)
+open FStar.Buffer
+(** Mathematical definitions *)
+open FStar.Math.Lemmas
+(** Helper functions for buffers *)
+open Buffer.Utils
+open Crypto.Symmetric.Bytes
+
+open FStar.Buffer.Quantifiers
+
+open Hacl.Symmetric.Poly1305_64.Parameters
+open Hacl.Symmetric.Poly1305_64.Bigint
+open Hacl.Symmetric.Poly1305_64.FC.Spec
+open Hacl.Symmetric.Poly1305_64.FC
+open Flag
+
+module U8  = FStar.UInt8
+module U32 = FStar.UInt32
+module U64 = FStar.UInt64
+module H8   = Hacl.UInt8
+module H64  = Hacl.UInt64
+module H128 = Hacl.UInt128
+module HS  = FStar.HyperStack
+
+
+#set-options "--initial_fuel 0 --max_fuel 0 --initial_ifuel 0 --max_ifuel 0 --z3timeout 20"
+
+// we may separate field operations, so that we don't
+// need to open the bignum modules elsewhere
+
+(* * *********************************************)
+(* *            Representation type              *)
+(* * *********************************************)
+
+(** Mutable big integer representation (5 64-bit limbs) *)
+type elemB = elemB //b:Buffer.buffer u64{length b == norm_length}
+
+(** Concrete (mutable) representation of words *)
+let wordB : Type0 = if mac_log then b:uint8_p{length b <= 16} else wordB
+let wordB_16 : Type0 = if mac_log then b:uint8_p{length b == 16} else wordB_16
+
+let word : Type0 = if mac_log then seq U8.t else seq H8.t
+(* let bytes : Type0 = if mac_log then Buffer.buffer U8.t else uint8_p *)
+
+(* * *********************************************)
+(* *  Mappings from stateful types to pure types *)
+(* * *********************************************)
+
+let live h (b:wordB) = if mac_log then live #U8.t h b else live #H8.t h b
+
+(** From the current memory state, returns the word corresponding to a wordB *)
+val sel_word: h:mem -> b:wordB{live h b} -> GTot word
+let sel_word h b = sel_word h b
+
+(** Only used when mac_log is true *)
+private val _read_word:
+  len:u32 ->
+  b:wordB{mac_log /\ length #U8.t b == U32.v len} ->
+  s:seq byte ->
+  i:u32{U32.v i <= U32.v len} ->
+  ST word
+    (requires (fun h -> live h b /\ Seq.slice (sel_word h b) 0 (U32.v i) == s))
+    (ensures  (fun h0 s h1 -> h0 == h1 /\ live h1 b /\ s == sel_word h1 b))
+let rec _read_word len b s i =
+  let h = ST.get () in
+  if U32.v i = U32.v len then
+    begin
+    Seq.lemma_eq_intro s (sel_word h b);
+    s
+    end
+  else
+    begin
+    let x = b.(i) in
+    let s' = FStar.Seq (s @| Seq.create 1 x) in
+    Seq.lemma_eq_intro s' (Seq.slice (sel_word h b) 0 (U32.v i + 1));
+    _read_word len b s' (U32 (i +^ 1ul))
+    end
+
+val read_word: len:u32 -> b:wordB{mac_log /\ length #U8.t b == U32.v len} -> ST word
+  (requires (fun h0 -> live h0 b))
+  (ensures (fun h0 r h1 -> h0 == h1 /\ live h1 b /\ r == (sel_word h1 b)))
+let read_word len b =
+  let h = ST.get() in
+  let s0 = Seq.createEmpty #byte in
+  Seq.lemma_eq_intro s0 (Seq.slice (sel_word h b) 0 0);
+  _read_word len b s0 0ul
+
+(** From the current memory state, returns the field element corresponding to a elemB *)
+val sel_elem: h:mem -> b:elemB{live h b} -> GTot elem
+let sel_elem h b = sel_elem h b
+
+(** From the current memory state, returns the integer corresponding to a elemB, (before
+   computing the modulo) *)
+val sel_int: h:mem -> b:elemB{live h b} -> GTot nat
+let sel_int h b = sel_int h b
+
+
+(* * ******************************************** *)
+(* *        Polynomial computation step           *)
+(* * ******************************************** *)
+
+(* Initialization function:
+   - clamps the first half of the key
+   - stores the well-formatted first half of the key in 'r' *)
+
+let log_t = if mac_log then Seq.seq elem else log_t
+
+
+val poly1305_encode_r:
+  r:bigint ->
+  key:uint8_p{length key = 16} ->
+  Stack unit
+    (requires (fun h -> live h r /\ live h key /\ disjoint key r))
+    (ensures  (fun h0 _ h1 -> modifies_1 r h0 h1 /\ live h1 r
+      // TODO: function correctness
+      ))
+let poly1305_encode_r r key =
+  poly1305_encode_r r key
+
+
+val poly1305_encode_b:
+  b:bigint ->
+  m:wordB_16 ->
+  Stack unit
+    (requires (fun h -> live h b /\ live h m /\ disjoint #H64.t #byte b m))
+    (ensures  (fun h0 _ h1 -> modifies_1 b h0 h1 /\ live h1 b))
+let poly1305_encode_b b m =
+  poly1305_encode_b b m
+
+
+val poly1305_init:
+  st:poly1305_state ->
+  key:uint8_p{length key >= 32 /\ disjoint st.r key} ->
+  Stack log_t
+    (requires (fun h -> live_st h st /\ live h key))
+    (ensures  (fun h0 log h1 -> live_st h0 st /\ live h0 key
+      (* /\ norm h1 r /\ live h1 s *)
+      (* /\ (if mac_log then modifies_2 #H64.t #U8.t r s h0 h1 else modifies_2 #H64.t #H8.t r s h0 h1) *)
+      /\ sel_int h1 st.r == Spec.clamp (sel_word h0 (sub key 0ul 16ul))))
+let poly1305_init st key =
+  poly1305_init st key
+
+
+(* val poly1305_start: acc:elemB -> Stack unit *)
+(*   (requires (fun h -> live h acc)) *)
+(*   (ensures  (fun h0 _ h1 -> modifies_1 acc h0 h1 *)
+(*     /\ norm h1 acc *)
+(*     /\ sel_elem h1 acc == 0)) *)
+(* let poly1305_start a = zeroB a *)
+
+
+(**
+   Update function:
+   - takes a ghost log
+   - takes a message block, appends '1' to it and formats it to bigint format
+   - runs acc = ((acc*block)+r) % p
+   *)
+
+//CF note the log now consists of elem
+//CF we'll need a simpler, field-only update---not the one below.
+
+val seq_head_snoc: #a:Type -> xs:Seq.seq a -> x:a ->
+  Lemma (Seq.length (SeqProperties.snoc xs x) > 0 /\
+         seq_head (SeqProperties.snoc xs x) == xs)
+let seq_head_snoc #a xs x =
+  Seq.lemma_len_append xs (Seq.create 1 x);
+  Seq.lemma_eq_intro (seq_head (SeqProperties.snoc xs x)) xs
+
+(* let log_t: Type0 = if mac_log then text else unit *)
+
+val ilog: l:log_t{mac_log} -> Tot text
+let ilog l = l
+
+val poly1305_update:
+  current_log:log_t ->
+  msg:wordB_16 ->
+  st:poly1305_state{
+    if mac_log then (disjoint #U8.t msg st.h /\ disjoint #U8.t msg st.r)
+    else (disjoint #H8.t msg st.h /\ disjoint #H8.t msg st.r)} ->
+  (* acc:elemB{if mac_log then disjoint #U8.t msg acc else disjoint #H8.t msg acc} ->  *)
+  (* r:elemB{if mac_log then disjoint #U8.t msg r else disjoint #H8.t msg r /\ disjoint acc r} ->  *)
+  Stack log_t
+  (requires (fun h -> live h msg /\ norm h st.h /\ norm h st.r
+    /\ (mac_log ==> sel_elem h (st.h) == poly (ilog current_log) (sel_elem h (st.r))) ))
+  (ensures (fun h0 updated_log h1 -> live h1 msg /\ norm h1 (st.h) /\ norm h1 (st.r)
+    /\ norm h0 (st.r)
+    /\ modifies_1 st.h h0 h1
+    /\ (mac_log ==>
+         ilog updated_log == SeqProperties.snoc (ilog current_log) (encode (sel_word h1 msg))
+       /\ sel_elem h1 st.h == poly (ilog updated_log) (sel_elem h0 st.r)) ))
+
+let elem : Type0 = if mac_log then elem else erased elem
+
+open FStar.SeqProperties
+
+(* let seq_bytes = if mac_log then Seq.seq U8.t else Seq.seq H8.t *)
+
+let rec little_endian (b:Seq.seq byte) : Tot (n:nat) (decreases (Seq.length b)) =
+  if Seq.length b = 0 then 0
+  else
+    UInt8.v (head b) + pow2 8 * little_endian (tail b)
+
+let encode (w:word) : Tot elem =
+  if mac_log
+    then (let l = Seq.length #U8.t w in
+          pow2_le_compat 128 (8*l);
+          pow2 (8 * l) +@ little_endian w)
+    else elift1 (fun w -> encode w) w
+
+#set-options "--z3timeout 60 --initial_fuel 1 --max_fuel 1"
+
+let poly1305_update log msgB st =
+  let m0 = ST.get () in
+  push_frame();
+  let r0 = st.r.(0ul) in
+  let r1 = st.r.(1ul) in
+  let r2 = st.r.(2ul) in
+  let five = Hacl.Cast.uint64_to_sint64 5uL in
+  let s1 = H64 (r1 *^ (five <<^ 2ul)) in
+  let s2 = H64 (r2 *^ (five <<^ 2ul)) in
+  let l = poly1305_update log st msgB r0 r1 r2 s1 s2 in
+  let updated_log:log_t =
+    if mac_log then
+      begin
+      let msg = read_word 16ul msgB in
+      (* assert (encode msg == sel_elem h1 block); *)
+      seq_head_snoc (ilog log) (encode msg);
+      Seq.lemma_index_app2 (ilog log) (Seq.create 1 (encode msg)) (Seq.length (SeqProperties.snoc (ilog log) (encode msg)) - 1);
+      SeqProperties.snoc (ilog log) (encode msg)
+      end
+    else l in
+  pop_frame();
+  let m3 = ST.get () in
+  (* eval_eq_lemma h2 h3 (st.h) (st.h) Hacl.Symmetric.Poly1305_64.Parameters.norm_length; *)
+  assert (norm m3 st.h);
+  assert (modifies_1 st.h m0 m3);
+  updated_log
+
+
+#set-options "--z3timeout 40 --initial_fuel 0 --max_fuel 0 --initial_ifuel 0 --max_ifuel 0"
+
+val append_as_seq_sub: h:HyperStack.mem -> n:UInt32.t -> m:UInt32.t -> msg:uint8_p{live h msg /\ U32.v m <= U32.v n /\ U32.v n <= length msg} -> Lemma
+  (append (as_seq h (Buffer.sub msg 0ul m))
+          (as_seq h (Buffer.sub (Buffer.offset msg m) 0ul (U32 (n -^ m)))) ==
+   as_seq h (Buffer.sub msg 0ul n))
+let append_as_seq_sub h n m msg =
+  Seq.lemma_eq_intro
+    (append (as_seq h (Buffer.sub msg 0ul m))
+            (as_seq h (Buffer.sub (Buffer.offset msg m) 0ul (U32 (n -^ m)))))
+     (as_seq h (Buffer.sub msg 0ul n))
+
+(* Loop over Poly1305_update; could go below MAC *)
+val poly1305_loop:
+  current_log:log_t ->
+  msg:uint8_p ->
+  (* acc:elemB{disjoint msg acc} -> *)
+  (* r:elemB{disjoint msg r /\ disjoint acc r} -> *)
+  st:poly1305_state ->
+  ctr:u32{length msg >= 16 * U32.v ctr} ->
+  ST log_t
+  (requires (fun h -> live h msg /\ norm h st.h /\ norm h st.r /\
+      (mac_log ==>
+        sel_elem h st.h == poly (ilog current_log) (sel_elem h st.r)) ))
+  (ensures (fun h0 updated_log h1 -> live h0 msg /\ norm h1 st.h /\ norm h0 st.r /\
+      modifies_1 st.h h0 h1 /\
+      (mac_log ==>
+        (ilog updated_log ==
+        encode_pad (ilog current_log) (as_seq h0 (Buffer.sub msg 0ul (UInt32.mul 16ul ctr))) /\
+        sel_elem h1 st.h == poly (ilog updated_log) (sel_elem h0 st.r))) ))
+    (decreases (U32.v ctr))
+#set-options "--z3timeout 100 --initial_fuel 0 --max_fuel 0 --initial_ifuel 0 --max_ifuel 0"
+let rec poly1305_loop log msg st ctr =
+  if mac_log then (
+    let h0 = ST.get() in
+    if U32.lte ctr 0ul then
+      begin
+        encode_pad_empty (ilog log) (as_seq h0 (Buffer.sub msg 0ul 0ul));
+        log
+      end
+    else
+      begin
+        let msg0:wordB_16 = Buffer.sub msg 0ul 16ul in
+        let log1 = poly1305_update log msg0 st in
+        let h1 = ST.get () in
+        let msg1 = Buffer.offset msg 16ul in
+        eval_eq_lemma h0 h1 st.r st.r norm_length;
+        assert (live h1 msg1 /\ norm h1 st.h /\ norm h1 st.r);
+        assert (mac_log ==> sel_elem h1 st.h == poly (ilog log1) (sel_elem h0 st.r));
+        assert (mac_log ==>
+          ilog log1 == SeqProperties.snoc (ilog log) (encode (sel_word h1 msg0)));
+        let log2 = poly1305_loop log1 msg1 st (U32 (ctr -^ 1ul)) in
+        let h2 = ST.get () in
+        assert (norm h2 st.h /\ modifies_1 st.h h0 h2);
+        lemma_modifies_1_trans st.h h0 h1 h2;
+        if mac_log then
+          begin
+          //assert (ilog log2 ==
+          //  encode_pad (ilog log1)
+          //    (as_seq h0 (Buffer.sub msg1 0ul (UInt32.mul 16ul (ctr -| 1ul)))) );
+          //assert (encode_pad (ilog log1)
+          //  (as_seq h0 (Buffer.sub msg1 0ul (UInt32.mul 16ul (ctr -| 1ul)))) ==
+          //encode_pad (SeqProperties.snoc (ilog log) (encode (sel_word h1 msg0)))
+          //  (as_seq h0 (Buffer.sub (Buffer.offset msg 16ul) 0ul (UInt32.mul 16ul ctr -| 16ul))));
+          encode_pad_snoc (ilog log) (as_seq h0 (Buffer.sub (Buffer.offset msg 16ul) 0ul (U32 (16ul *^ ctr -^ 16ul)))) (sel_word h1 msg0);
+          append_as_seq_sub h0 (UInt32.mul 16ul ctr) 16ul msg
+          //assert (append (sel_word h1 msg0) (as_seq h0 (Buffer.sub (Buffer.offset msg 16ul) 0ul  (UInt32.mul 16ul ctr -| 16ul))) ==
+          // (as_seq h0 (Buffer.sub msg 0ul (UInt32.mul 16ul ctr))))
+          end;
+        log2
+      end)
+  else poly1305_blocks_loop log st msg
+
+(**
+   Performs the last step if there is an incomplete block
+   NB: Not relevant for AEAD-ChachaPoly which only uses complete blocks of 16 bytes, hence
+   only the 'update' and 'loop' functions are necessary there
+*)
+val poly1305_last:
+  current_log:log_t ->
+  msg:wordB ->
+  (* acc:elemB{disjoint msg acc} -> *)
+  (* r:elemB{disjoint msg r /\ disjoint acc r} ->  *)
+  st:poly1305_state ->
+  len:u32{U32.v len == (if mac_log then length #U8.t msg else length #H8.t msg)
+    /\ 0 < U32.v len /\ U32.v len < 16} ->
+  Stack log_t
+    (requires (fun h -> live h msg /\ norm h st.h /\ norm h st.r
+      /\ (mac_log ==> sel_elem h st.h == poly (ilog current_log) (sel_elem h st.r)) ))
+    (ensures (fun h0 updated_log h1 -> live h1 msg /\ norm h1 st.h /\ norm h1 st.r
+      /\ norm h0 st.r
+      /\ modifies_1 st.h h0 h1
+      /\ (mac_log ==>
+           ilog updated_log == SeqProperties.snoc (ilog current_log) (encode (sel_word h1 msg))
+         /\ sel_elem h1 st.h == poly (ilog updated_log) (sel_elem h0 st.r)) ))
+
+#set-options "--z3timeout 60 --initial_fuel 1 --max_fuel 1"
+
+let poly1305_last log msg st len =
+  let m0 = ST.get() in
+  let log = poly1305_last log st msg (Int.Cast.uint32_to_uint64 len) in
+  let updated_log:log_t =
+    if mac_log then
+      begin
+      let msg = read_word len msg in
+      (* assert (encode msg == sel_elem h1 block); *)
+      seq_head_snoc (ilog log) (encode msg);
+      Seq.lemma_index_app2 (ilog log) (Seq.create 1 (encode msg)) (Seq.length (SeqProperties.snoc (ilog log) (encode msg)) - 1);
+      SeqProperties.snoc (ilog log) (encode msg)
+      end
+    else () in
+  pop_frame ();
+  let m3 = ST.get() in
+  (* eval_eq_lemma h2 h3 acc acc Parameters.norm_length; *)
+  assert (norm m3 st.h);
+  assert (modifies_1 st.h m0 m3);
+  updated_log
+
+
+(* (\* TODO: certainly a more efficient, better implementation of that *\) *)
+(* private val add_word: a:wordB_16 -> b:wordB_16 -> Stack unit *)
+(*   (requires (fun h -> live h a /\ live h b)) *)
+(*   (ensures  (fun h0 _ h1 -> live h0 a /\ live h0 b /\ live h1 a /\ modifies_1 a h0 h1 /\ *)
+(*      little_endian (sel_word h1 a) == *)
+(*      (little_endian (sel_word h0 a) + little_endian (sel_word h0 b)) % pow2 128 )) *)
+(* let add_word a b = *)
+(*   let carry = 0ul in *)
+(*   let a04:u64 = let (x:u32) = uint32_of_bytes a in uint32_to_uint64 x  in *)
+(*   let a48:u64 = let (x:u32) = uint32_of_bytes (offset a 4ul) in uint32_to_uint64 x in *)
+(*   let a812:u64 = let (x:u32) = uint32_of_bytes (offset a 8ul) in uint32_to_uint64 x in *)
+(*   let a1216:u64 = let (x:u32) = uint32_of_bytes (offset a 12ul) in uint32_to_uint64 x in *)
+(*   let b04:u64 = let (x:u32) = uint32_of_bytes b in uint32_to_uint64 x  in *)
+(*   let b48:u64 = let (x:u32) = uint32_of_bytes (offset b 4ul) in uint32_to_uint64 x in *)
+(*   let b812:u64 = let (x:u32) = uint32_of_bytes (offset b 8ul) in uint32_to_uint64 x in *)
+(*   let b1216:u64 = let (x:u32) = uint32_of_bytes (offset b 12ul) in uint32_to_uint64 x in *)
+(*   let open FStar.UInt64 in *)
+(*   let z0 = a04 +^ b04 in *)
+(*   let z1 = a48 +^ b48 +^ (z0 >>^ 32ul) in *)
+(*   let z2 = a812 +^ b812 +^ (z1 >>^ 32ul) in *)
+(*   let z3 = a1216 +^ b1216 +^ (z2 >>^ 32ul) in *)
+(*   bytes_of_uint32 (Buffer.sub a 0ul 4ul) (uint64_to_uint32 z0); *)
+(*   bytes_of_uint32 (Buffer.sub a 4ul 4ul) (uint64_to_uint32 z1); *)
+(*   bytes_of_uint32 (Buffer.sub a 8ul 4ul) (uint64_to_uint32 z2); *)
+(*   bytes_of_uint32 (Buffer.sub a 12ul 4ul) (uint64_to_uint32 z3); *)
+(*   admit () *)
+
+(* Finish function, with final accumulator value *)
+val poly1305_finish:
+  log:log_t ->
+  tag:wordB_16 ->
+  st:poly1305_state ->
+  key:uint8_p ->
+  (* acc:elemB -> *)
+  (* s:wordB_16 -> *)
+  ST unit
+    (requires (fun h -> live h tag /\ live h st.h /\ live h key
+      /\ norm h st.h
+      /\ (if mac_log then disjoint #U8.t tag st.h else disjoint #H8.t tag st.h)
+      /\ (if mac_log then disjoint #U8.t tag key else disjoint #H8.t tag key)
+      /\ disjoint st.h key))
+    (ensures  (fun h0 _ h1 -> live h0 st.h /\ live h0 key
+      /\ (if mac_log then modifies_2 #U8.t tag st.h h0 h1 else modifies_2 #H8.t tag st.h h0 h1)
+      /\ live h1 st.h /\ live h1 tag
+      /\ little_endian (sel_word h1 tag) ==
+        (trunc_1305 (sel_elem h0 st.h) + little_endian (sel_word h0 key)) % pow2 128))
+let poly1305_finish log tag st key =
+  let _ = poly1305_last_sum log st tag key in
+  ()
+
+val div_aux: a:UInt32.t -> b:UInt32.t{U32.v b <> 0} -> Lemma
+  (requires True)
+  (ensures FStar.UInt32(UInt.size (v a / v b) n))
+  [SMTPat (FStar.UInt32(UInt.size (v a / v b) n))]
+let div_aux a b = ()
+
+(** Computes the Poly1305 MAC on a buffer *)
+val poly1305_mac:
+  tag:wordB{if mac_log then length #U8.t tag == 16 else length #H8.t tag == 16} ->
+  msg:uint8_p{if mac_log then disjoint #U8.t tag msg else disjoint #H8.t tag msg} ->
+  len:u32{U32.v len == length msg} ->
+  key:uint8_p{length key == 32 /\ disjoint msg key
+    /\ (if mac_log then disjoint #U8.t tag key else disjoint #H8.t tag key)} ->
+  Stack unit
+    (requires (fun h -> live h msg /\ live h key /\ live h tag))
+    (ensures (fun h0 _ h1 -> live h0 msg /\ live h0 key /\ live h1 tag
+      /\ (if mac_log then modifies_1 #U8.t tag h0 h1 else modifies_1 #H8.t tag h0 h1)
+      /\ (let r = Spec.clamp (sel_word h0 (sub key 0ul 16ul)) in
+         let s = sel_word h0 (sub key 16ul 16ul) in
+         little_endian (sel_word h1 tag) ==
+         mac_1305 (encode_pad Seq.createEmpty (Buffer.as_seq h0 msg)) r s)))
+let poly1305_mac tag msg len key =
+  let h0 = ST.get () in
+  push_frame();
+  (* Create buffers for the 2 parts of the key and the accumulator *)
+  (* let tmp = create 0UL 10ul in *)
+  (* let acc = sub tmp 0ul 5ul in *)
+  (* let r   = sub tmp 5ul 5ul in *)
+  (* let s   = create 0uy 16ul in *)
+  let tmp = create (Hacl.Cast.uint64_to_sint64 0uL) 6ul in
+  let r = sub tmp 0ul 3ul in
+  let h = sub tmp 3ul 3ul in
+  let st = {r = r; h = h} in
+  (* Initializes the accumulator and the keys values *)
+  let initial_log = poly1305_init st key in
+  (* let h1 = ST.get () in *)
+  (* assert (sel_int h1 r == Spec.clamp (sel_word h0 (sub key 0ul 16ul))); *)
+  (* assert (sel_word h1 s == sel_word h0 (sub key 16ul 16ul)); *)
+  (* poly1305_start acc; // zeroes acc redundantly *)
+  (* Compute the number of 'plain' blocks *)
+  let ctr = U32.div len 16ul in
+  let rest = U32.rem len 16ul in
+  (* Run the poly1305_update function ctr times *)
+  let l:log_t = if mac_log then Seq.createEmpty #elem else () in
+  let h2 = ST.get () in
+  (* norm_eq_lemma h1 h2 r r; *)
+  let l = poly1305_loop l msg st ctr in
+  assume False; // TODO: REMOVE ME
+  (* Run the poly1305_update function one more time on the last incomplete block *)
+  let last_block = sub msg (FStar.UInt32 (ctr *^ 16ul)) rest in
+  let l = poly1305_last l last_block st rest in
+  (* Finish *)
+  poly1305_finish l tag st (sub key 16ul 16ul);
+  pop_frame()
