examples/low-level/crypto/Hacl.Symmetric.Poly1305_64.FC.Spec.fst
@@ -1,0 +1,381 @@
+module Hacl.Symmetric.Poly1305_64.FC.Spec
+
+open FStar.Mul
+open FStar.ST
+
+open Hacl.Cast
+
+open Hacl.Symmetric.Poly1305_64.Parameters
+open Hacl.Symmetric.Poly1305_64.Bigint
+
+
+module H8   = Hacl.UInt8
+module H64  = Hacl.UInt64
+module H128 = Hacl.UInt128
+module U8   = FStar.UInt8
+module U64  = FStar.UInt64
+module U128 = FStar.UInt64
+
+open FStar.Ghost
+
+let p_1305: p:nat{pow2 128 < p} =
+  assert_norm (pow2 128 < pow2 130 - 5);
+  pow2 130 - 5
+
+type elem = n:nat{n < p_1305}
+type word = b:Seq.seq H8.byte{Seq.length b <= 16}
+type word_16 = b:Seq.seq H8.byte{Seq.length b = 16}
+type text = Seq.seq elem
+type tag  = word_16
+
+val field_add: elem -> elem -> Tot elem
+let field_add a b = (a + b) % p_1305
+val field_mul: elem -> elem -> Tot elem
+let field_mul a b = (a * b) % p_1305
+
+(* Infix field operators for readability *)
+let op_Plus_At = field_add
+let op_Star_At = field_mul
+
+
+(* * *********************************************)
+(* *            Encoding                         *)
+(* * *********************************************)
+
+open FStar.Math.Lemmas
+open FStar.SeqProperties
+
+let bytes = Seq.seq H8.t
+
+(* Little endian integer value of a sequence of bytes *)
+let rec little_endian (b:Seq.seq H8.t) : GTot (n:nat) (decreases (Seq.length b)) =
+  if Seq.length b = 0 then 0
+  else
+    H8.v (head b) + pow2 8 * little_endian (tail b)
+
+
+#reset-options "--initial_fuel 1 --max_fuel 1 --z3timeout 20"
+
+let zerob = uint8_to_sint8 0uy
+
+val little_endian_null: len:nat{len < 16} -> Lemma
+  (little_endian (Seq.create len (uint8_to_sint8 0uy)) == 0)
+let rec little_endian_null len =
+  if len = 0 then ()
+  else
+    begin
+    Seq.lemma_eq_intro (Seq.slice (Seq.create len zerob) 1 len)
+		       (Seq.create (len - 1) zerob);
+    assert (little_endian (Seq.create len zerob) ==
+      0 + pow2 8 * little_endian (Seq.slice (Seq.create len zerob) 1 len));
+    little_endian_null (len - 1)
+    end
+
+val little_endian_singleton: n:H8.t -> Lemma
+  (little_endian (Seq.create 1 n) == H8.v n)
+let little_endian_singleton n =
+  assert (little_endian (Seq.create 1 n) ==
+    H8.v (Seq.index (Seq.create 1 n) 0) + pow2 8 *
+    little_endian (Seq.slice (Seq.create 1 n) 1 1))
+
+
+val little_endian_append: w1:bytes -> w2:bytes -> Lemma
+  (requires True)
+  (ensures
+    little_endian (Seq.append w1 w2) ==
+    little_endian w1 + pow2 (8 * Seq.length w1) * little_endian w2)
+  (decreases (Seq.length w1))
+let rec little_endian_append w1 w2 =
+  let open FStar.Seq in
+  if length w1 = 0 then
+    begin
+    assert_norm (pow2 (8 * 0) == 1);
+    Seq.lemma_eq_intro (append w1 w2) w2
+    end
+  else
+    begin
+    let w1' = slice w1 1 (length w1) in
+    assert (length w1' == length w1 - 1);
+    little_endian_append w1' w2;
+    assert (index (append w1 w2) 0 == index w1 0);
+    Seq.lemma_eq_intro
+      (append w1' w2)
+      (Seq.slice (append w1 w2) 1 (length (append w1 w2)));
+    assert (little_endian (append w1 w2) ==
+      H8.v (index w1 0) + pow2 8 * little_endian (append w1' w2));
+    assert (little_endian (append w1' w2) ==
+      little_endian w1' + pow2 (8 * length w1') * little_endian w2);
+    assert (H8.v (index w1 0) + pow2 8 * little_endian (append w1' w2) ==
+      H8.v (index w1 0) +
+      pow2 8 * (little_endian w1' + pow2 (8 * length w1') * little_endian w2));
+    Math.Lemmas.pow2_plus 8 (8 * (length w1 - 1));
+    assert (pow2 8 * pow2 (8 * length w1') == pow2 (8 * length w1));
+    assert (H8.v (index w1 0) + pow2 8 * little_endian (append w1' w2) ==
+      H8.v (index w1 0) +
+      pow2 8 * little_endian w1' + pow2 (8 * length w1) * little_endian w2);
+    assert (H8.v (index w1 0) + pow2 8 * little_endian w1' == little_endian w1)
+    end
+
+private val lemma_factorise: a:nat -> b:nat -> Lemma (a + a * b == a * (b + 1))
+let lemma_factorise a b = ()
+
+val lemma_euclidean_division: r:nat -> b:nat -> q:pos -> Lemma
+  (requires (r < q))
+  (ensures  (r + q * b < q * (b+1)))
+let lemma_euclidean_division r b q = ()
+
+val lemma_little_endian_is_bounded: b:bytes -> Lemma
+  (requires True)
+  (ensures  (little_endian b < pow2 (8 * Seq.length b)))
+  (decreases (Seq.length b))
+let rec lemma_little_endian_is_bounded b =
+  if Seq.length b = 0 then ()
+  else
+    begin
+    let s = Seq.slice b 1 (Seq.length b) in
+    assert(Seq.length s = Seq.length b - 1);
+    lemma_little_endian_is_bounded s;
+    assert(H8.v (Seq.index b 0) < pow2 8);
+    assert(little_endian s < pow2 (8 * Seq.length s));
+    assert(little_endian b < pow2 8 + pow2 8 * pow2 (8 * (Seq.length b - 1)));
+    lemma_euclidean_division (H8.v (Seq.index b 0)) (little_endian s) (pow2 8);
+    assert(little_endian b <= pow2 8 * (little_endian s + 1));
+    assert(little_endian b <= pow2 8 * pow2 (8 * (Seq.length b - 1)));
+    Math.Lemmas.pow2_plus 8 (8 * (Seq.length b - 1));
+    lemma_factorise 8 (Seq.length b - 1)
+    end
+
+#reset-options "--initial_fuel 0 --max_fuel 0"
+
+val lemma_little_endian_lt_2_128: b:bytes {Seq.length b <= 16} -> Lemma
+  (requires True)
+  (ensures  (little_endian b < pow2 128))
+  [SMTPat (little_endian b)]
+let lemma_little_endian_lt_2_128 b =
+  lemma_little_endian_is_bounded b;
+  if Seq.length b = 16 then ()
+  else Math.Lemmas.pow2_lt_compat 128 (8 * Seq.length b)
+
+
+let encode (w:word) : GTot elem =
+  let l = Seq.length w in
+  pow2_le_compat 128 (8 * l);
+  pow2 (8 * l) +@ little_endian w
+
+
+val encode_pad: prefix:Seq.seq elem -> txt:Seq.seq H8.t -> GTot (Seq.seq elem) 
+  (decreases (Seq.length txt))
+let rec encode_pad prefix txt =
+  let l = Seq.length txt in
+  if l = 0 then prefix
+  else if l < 16 then
+    let w = txt in
+    SeqProperties.snoc prefix (encode w)
+  else
+    begin
+    let w, txt = SeqProperties.split txt 16 in
+    let prefix = SeqProperties.snoc prefix (encode w) in
+    encode_pad prefix txt
+    end
+
+
+let trunc_1305 (e:elem) : Tot elem = e % pow2 128
+
+(* * *********************************************)
+(* *          Encoding-related lemmas            *)
+(* * *********************************************)
+
+#reset-options "--initial_fuel 1 --max_fuel 1 --initial_ifuel 0 --max_ifuel 0"
+
+
+#reset-options "--initial_fuel 1 --max_fuel 1 --initial_ifuel 0 --max_ifuel 0"
+
+open FStar.Math.Lib
+open FStar.Math.Lemmas
+
+val lemma_little_endian_is_injective_0: b:word{Seq.length b > 0} -> Lemma
+  (little_endian b =
+   H8.v (Seq.index b 0) + pow2 8 * little_endian (Seq.slice b 1 (Seq.length b)))
+let lemma_little_endian_is_injective_0 b = ()
+
+val lemma_little_endian_is_injective_1: b:pos -> q:nat -> r:nat -> q':nat -> r':nat -> Lemma
+  (requires (r < b /\ r' < b /\ r + b * q = r' + b * q'))
+  (ensures  (r = r' /\ q = q'))
+let lemma_little_endian_is_injective_1 b q r q' r' =
+  lemma_mod_plus r q b;
+  lemma_mod_plus r' q' b;
+  lemma_mod_injective b r r'
+
+val lemma_little_endian_is_injective_2: b:word -> len:pos{len <= Seq.length b} -> Lemma
+  (let s = Seq.slice b (Seq.length b - len) (Seq.length b) in
+   let s' = Seq.slice s 1 (Seq.length s) in
+   let s'' = Seq.slice b (Seq.length b - (len - 1)) (Seq.length b) in
+   s'' == s')
+let lemma_little_endian_is_injective_2 b len =
+  let s = Seq.slice b (Seq.length b - len) (Seq.length b) in
+  let s' = Seq.slice s 1 (Seq.length s) in
+  let s'' = Seq.slice b (Seq.length b - (len - 1)) (Seq.length b) in
+  Seq.lemma_eq_intro s' s''
+
+val lemma_little_endian_is_injective_3: b:word -> b':word -> len:pos{len <= Seq.length b /\ len <= Seq.length b'} -> Lemma
+  (requires (Seq.slice b (Seq.length b - (len - 1)) (Seq.length b) ==
+             Seq.slice b' (Seq.length b' - (len-1)) (Seq.length b')
+           /\ Seq.index b (Seq.length b - len) = Seq.index b' (Seq.length b' - len)))
+  (ensures  (Seq.slice b (Seq.length b - len) (Seq.length b) ==
+             Seq.slice b' (Seq.length b' - len) (Seq.length b')))
+let lemma_little_endian_is_injective_3 b b' len =
+  Seq.lemma_eq_intro (Seq.slice b' (Seq.length b' - len) (Seq.length b'))
+                     (Seq.append (Seq.create 1 (Seq.index b' (Seq.length b' - len))) (Seq.slice b' (Seq.length b' - (len-1)) (Seq.length b')));
+  Seq.lemma_eq_intro (Seq.slice b (Seq.length b - len) (Seq.length b))
+                     (Seq.append (Seq.create 1 (Seq.index b (Seq.length b - len))) (Seq.slice b (Seq.length b - (len-1)) (Seq.length b)))
+
+val lemma_little_endian_is_injective: b:word -> b':word ->
+  len:nat{Seq.length b >= len /\ Seq.length b' >= len} -> Lemma
+  (requires (little_endian (Seq.slice b (Seq.length b - len) (Seq.length b)) =
+             little_endian (Seq.slice b' (Seq.length b' - len) (Seq.length b')) ))
+  (ensures  (Seq.slice b (Seq.length b - len) (Seq.length b) ==
+             Seq.slice b' (Seq.length b' - len) (Seq.length b')))
+let rec lemma_little_endian_is_injective b b' len =
+  if len = 0 then
+    Seq.lemma_eq_intro (Seq.slice b (Seq.length b - len) (Seq.length b))
+                       (Seq.slice b' (Seq.length b' - len) (Seq.length b'))
+  else
+    begin
+    let s = Seq.slice b (Seq.length b - len) (Seq.length b) in
+    let s' = Seq.slice b' (Seq.length b' - len) (Seq.length b') in
+    assert(Seq.length s = len /\ Seq.length s' = len);
+    lemma_little_endian_is_injective_0 s; lemma_little_endian_is_injective_0 s';
+    lemma_little_endian_is_injective_1 (pow2 8)
+                                      (little_endian (Seq.slice s 1 (Seq.length s)))
+                                      (H8.v (Seq.index s 0))
+                                      (little_endian (Seq.slice s' 1 (Seq.length s')))
+                                      (H8.v (Seq.index s' 0));
+    lemma_little_endian_is_injective_2 b len;
+    lemma_little_endian_is_injective_2 b' len;
+    lemma_little_endian_is_injective b b' (len - 1);
+    lemma_little_endian_is_injective_3 b b' len
+    end
+
+val lemma_encode_injective: w0:word -> w1:word -> Lemma
+  (requires (Seq.length w0 == Seq.length w1 /\ encode w0 == encode w1))
+  (ensures  (w0 == w1))
+let lemma_encode_injective w0 w1 =
+  let l = Seq.length w0 in
+  lemma_little_endian_is_bounded w0;
+  lemma_little_endian_is_bounded w1;
+  pow2_le_compat 128 (8 * l);
+  lemma_mod_plus_injective p_1305 (pow2 (8 * l))
+    (little_endian w0) (little_endian w1);
+  assert (little_endian w0 == little_endian w1);
+  Seq.lemma_eq_intro (Seq.slice w0 0 l) w0;
+  Seq.lemma_eq_intro (Seq.slice w1 0 l) w1;
+  lemma_little_endian_is_injective w0 w1 l
+
+val lemma_encode_pad_injective: p0:Seq.seq elem -> t0:Seq.seq H8.t -> p1:Seq.seq elem -> t1:Seq.seq H8.t -> Lemma
+  (requires Seq.length t0 == Seq.length t1 /\ encode_pad p0 t0 == encode_pad p1 t1)
+  (ensures  p0 == p1 /\ t0 == t1)
+  (decreases (Seq.length t0))
+let rec lemma_encode_pad_injective p0 t0 p1 t1 =
+  let l = Seq.length t0 in
+  if l = 0 then Seq.lemma_eq_intro t0 t1
+  else if l < 16 then
+    begin
+    SeqProperties.lemma_append_inj
+      p0 (Seq.create 1 (encode t0))
+      p1 (Seq.create 1 (encode t1));
+    Seq.lemma_index_create 1 (encode t0) 0;
+    Seq.lemma_index_create 1 (encode t1) 0;
+    lemma_encode_injective t0 t1
+    end
+  else
+    begin
+    let w0, t0' = SeqProperties.split_eq t0 16 in
+    let w1, t1' = SeqProperties.split_eq t1 16 in
+    let p0' = SeqProperties.snoc p0 (encode w0) in
+    let p1' = SeqProperties.snoc p1 (encode w1) in
+    assert (encode_pad p0' t0' == encode_pad p1' t1');
+    lemma_encode_pad_injective p0' t0' p1' t1';
+    SeqProperties.lemma_append_inj
+      p0 (Seq.create 1 (encode w0))
+      p1 (Seq.create 1 (encode w1));
+    Seq.lemma_index_create 1 (encode w0) 0;
+    Seq.lemma_index_create 1 (encode w1) 0;
+    lemma_encode_injective w0 w1
+    end
+
+val encode_pad_empty: prefix:Seq.seq elem -> txt:Seq.seq H8.t -> Lemma
+  (requires Seq.length txt == 0)
+  (ensures  encode_pad prefix txt == prefix)
+let encode_pad_empty prefix txt = ()
+
+val encode_pad_snoc: prefix:Seq.seq elem -> txt:Seq.seq H8.t -> w:word_16 -> Lemma
+  (encode_pad (SeqProperties.snoc prefix (encode w)) txt ==
+   encode_pad prefix (Seq.append w txt))
+let encode_pad_snoc prefix txt w =
+  Seq.lemma_len_append w txt;
+  assert (16 <= Seq.length (Seq.append w txt));
+  let w', txt' = SeqProperties.split (Seq.append w txt) 16 in
+  let prefix' = SeqProperties.snoc prefix (encode w') in
+  Seq.lemma_eq_intro w w';
+  Seq.lemma_eq_intro txt txt'
+
+(* * *********************************************)
+(* *        Poly1305 functional invariant        *)
+(* * *********************************************)
+
+let seq_head (vs:Seq.seq 'a {Seq.length vs > 0}) = Seq.slice vs 0 (Seq.length vs - 1)
+
+val poly: vs:Seq.seq elem -> r:elem -> Tot (a:elem) (decreases (Seq.length vs))
+let rec poly vs r =
+  if Seq.length vs = 0 then 0
+  else (poly (seq_head vs) r +@ Seq.index vs (Seq.length vs - 1)) *@ r
+
+let log_t : Type0 = erased (Seq.seq elem)
+
+(* the definition above captures what POLY1305 does, 
+   not the usual polynomial computation; 
+   it may be more natural to flip the sequence, 
+   so that the coefficients are aligned. 
+   (i.e. a_0::a_1::a_2 stands for a_0 + a_1 X + a_2 X^2 , is implicitly extended with 0s.) *)
+
+val poly': vs:Seq.seq elem -> r:elem -> Tot (a:elem) (decreases (Seq.length vs))
+let rec poly' vs r =
+  if Seq.length vs = 0 then 0
+  else (SeqProperties.head vs +@ poly' (SeqProperties.tail vs) r ) *@ r
+
+val eq_poly0: p:Seq.seq elem -> Tot bool (decreases (Seq.length p)) 
+let rec eq_poly0 p = 
+  Seq.length p = 0 || 
+  (SeqProperties.head p = 0 && eq_poly0 (SeqProperties.tail p))
+  
+val eq_poly: p0:Seq.seq elem -> p1:Seq.seq elem -> Tot bool (decreases (Seq.length p0))
+let rec eq_poly p0 p1 = 
+  if Seq.length p0 = 0 then eq_poly0 p1 
+  else if Seq.length p1 = 0 then eq_poly0 p0
+  else SeqProperties.head p0 = SeqProperties.head p1 && eq_poly (SeqProperties.tail p0) (SeqProperties.tail p1)
+
+private let fix (r:word_16) (i:nat {i < 16}) m : Tot word_16 =
+  Seq.upd r i (H8 (Seq.index r i &^ m))
+
+// an abstract spec of clamping for our state invariant
+// for our polynomial-sampling assumption,
+// we rely solely on the number of fixed bits (22, right?)
+val clamp: word_16 -> GTot elem
+let clamp r =
+  assert_norm(pow2 8 > 15);
+  assert_norm(pow2 8 > 252);
+  let fifteen = uint8_to_sint8 15uy in
+  let thft = uint8_to_sint8 252uy in
+  let r = fix r  3  fifteen in // 0000****
+  let r = fix r  7  fifteen in
+  let r = fix r 11  fifteen in
+  let r = fix r 15  fifteen in
+  let r = fix r  4 thft in // ******00
+  let r = fix r  8 thft in
+  let r = fix r 12 thft in
+  little_endian r
+
+(** REMARK: this is equivalent to (poly vs r + little_endian s) % pow2 128 *)
+val mac_1305: vs:Seq.seq elem -> r:elem -> s:Seq.seq H8.t -> GTot int
+let mac_1305 vs r s = (trunc_1305 (poly vs r) + little_endian s) % pow2 128
+
