examples/low-level/crypto/Hacl.Symmetric.Poly1305_64.fst
@@ -1,0 +1,461 @@
+module Hacl.Symmetric.Poly1305_64
+
+open FStar.Mul
+open FStar.ST
+open FStar.Ghost
+open FStar.Seq
+open FStar.Buffer
+
+open Hacl.Cast
+
+open Hacl.Symmetric.Poly1305_64.Parameters
+open Hacl.Symmetric.Poly1305_64.Bigint
+
+open Hacl.Symmetric.Poly1305_64.FC.Spec
+open Hacl.Symmetric.Poly1305_64.FC
+
+
+module H8   = Hacl.UInt8
+module H64  = Hacl.UInt64
+module H128 = Hacl.UInt128
+module U8   = FStar.UInt8
+module U32  = FStar.UInt32
+module U64  = FStar.UInt64
+
+
+
+(*
+#reset-options "--initial_fuel 0 --max_fuel 0 --z3timeout 5"
+
+val pow2_8_lemma: n:nat ->
+  Lemma
+    (requires (n = 8))
+    (ensures  (pow2 n = 256))
+    [SMTPat (pow2 n)]
+let pow2_8_lemma n = assert_norm(pow2 8 = 256)
+
+val pow2_32_lemma: n:nat ->
+  Lemma
+    (requires (n = 32))
+    (ensures  (pow2 n = 4294967296))
+    [SMTPat (pow2 n)]
+let pow2_32_lemma n = assert_norm(pow2 32 = 4294967296)
+
+val pow2_64_lemma: n:nat ->
+  Lemma
+    (requires (n = 64))
+    (ensures  (pow2 n = 18446744073709551616))
+    [SMTPat (pow2 n)]
+let pow2_64_lemma n = assert_norm(pow2 64 = 18446744073709551616)
+
+let elemB = b:bigint
+
+let wordB = b:uint8_p{length b <= 16}
+let wordB_16 = b:uint8_p{length b = 16}
+
+noeq type poly1305_state = {
+  r:bigint;
+  h:bigint;
+  }
+
+val load64_le:
+  b:uint8_p{length b >= 8} ->
+  Stack h64
+    (requires (fun h -> live h b))
+    (ensures  (fun h0 _ h1 -> h0 == h1))
+let load64_le b =
+  let b0 = b.(0ul) in
+  let b1 = b.(1ul) in
+  let b2 = b.(2ul) in
+  let b3 = b.(3ul) in
+  let b4 = b.(4ul) in
+  let b5 = b.(5ul) in
+  let b6 = b.(6ul) in
+  let b7 = b.(7ul) in
+  H64 (
+    sint8_to_sint64 b0
+    |^ (sint8_to_sint64 b1 <<^ 8ul)
+    |^ (sint8_to_sint64 b2 <<^ 16ul)
+    |^ (sint8_to_sint64 b3 <<^ 24ul)
+    |^ (sint8_to_sint64 b4 <<^ 32ul)
+    |^ (sint8_to_sint64 b5 <<^ 40ul)
+    |^ (sint8_to_sint64 b6 <<^ 48ul)
+    |^ (sint8_to_sint64 b7 <<^ 56ul)
+  )
+
+
+val store64_le:
+  b:uint8_p{length b >= 8} ->
+  z:H64.t ->
+  Stack unit
+    (requires (fun h -> live h b))
+    (ensures  (fun h0 _ h1 -> modifies_1 b h0 h1 /\ live h1 b))
+let store64_le b z =
+  let open Hacl.UInt64 in
+  b.(0ul) <- sint64_to_sint8 z;
+  b.(1ul) <- sint64_to_sint8 (z >>^ 8ul);
+  b.(2ul) <- sint64_to_sint8 (z >>^ 16ul);
+  b.(3ul) <- sint64_to_sint8 (z >>^ 24ul);
+  b.(4ul) <- sint64_to_sint8 (z >>^ 32ul);
+  b.(5ul) <- sint64_to_sint8 (z >>^ 40ul);
+  b.(6ul) <- sint64_to_sint8 (z >>^ 48ul);
+  b.(7ul) <- sint64_to_sint8 (z >>^ 56ul)
+
+
+let live_st h (st:poly1305_state) : Type0 =
+  live h st.h /\ live h st.r /\ disjoint st.h st.r
+
+
+val poly1305_init:
+  st:poly1305_state ->
+  key:uint8_p{length key = 32} ->
+  Stack log_t
+    (requires (fun h -> live_st h st /\ live h key))
+    (ensures  (fun h0 _ h1 -> modifies_2 st.r st.h h0 h1 /\ live_st h1 st))
+let poly1305_init st key =
+  let t0 = load64_le(key) in
+  let t1 = load64_le(offset key 8ul) in
+
+  let open Hacl.UInt64 in
+  st.r.(0ul) <- ( t0                           ) &^ uint64_to_sint64 0xffc0fffffffuL;
+  st.r.(1ul) <- ((t0 >>^ 44ul) |^ (t1 <<^ 20ul)) &^ uint64_to_sint64 0xfffffc0ffffuL;
+  st.r.(2ul) <- ((t1 >>^ 24ul)                 ) &^ uint64_to_sint64 0x00ffffffc0fuL;
+
+  let zero = uint64_to_sint64 0uL in
+  st.h.(0ul) <- zero;
+  st.h.(1ul) <- zero;
+  st.h.(2ul) <- zero;
+  Ghost.hide (Seq.createEmpty #elem)
+
+
+let eval_3_limbs (h0:H64.t) (h1:H64.t) (h2:H64.t) : GTot nat =
+  let open Hacl.UInt64 in
+  Math.Lemmas.nat_times_nat_is_nat (pow2 44) (v h1);
+  Math.Lemmas.nat_times_nat_is_nat (pow2 88) (v h2);
+  (v h0 + pow2 44 * v h1 + pow2 88 * v h2) % prime
+
+
+let limb_44 = x:h64{H64.v x < pow2 44}
+let limb_45 = x:h64{H64.v x < pow2 45}
+let limb_44_20 = x:h64{H64.v x < 20 * pow2 44}
+
+
+val mk_mask: nbits:U32.t{U32.v nbits < 64} -> Tot (z:h64{H64.v z = pow2 (U32.v nbits) - 1})
+let mk_mask nbits =
+  admit();
+  let one = uint64_to_sint64 1uL in
+  H64 ((one <<^ nbits) -^ one)
+
+open FStar.HyperStack
+
+val sel_word:
+  h:mem ->
+  b:wordB{live h b} ->
+  GTot (s:Seq.seq H8.t{Seq.length s = length b
+    /\ (forall (i:nat). {:pattern (Seq.index s i)}
+      i < Seq.length s ==> H8.v (Seq.index s i) == H8.v (get h b i))})
+let sel_word h b = as_seq h b
+
+(** From the current memory state, returns the field element corresponding to a elemB *)
+val sel_elem: h:mem -> b:elemB{live h b} -> GTot elem
+let sel_elem h b = eval h b norm_length % p_1305
+
+(** From the current memory state, returns the integer corresponding to a elemB, (before
+   computing the modulo) *)
+val sel_int: h:mem -> b:elemB{live h b} -> GTot nat
+let sel_int h b = eval h b norm_length
+
+#reset-options "--z3timeout 20 --initial_fuel 0 --max_fuel 0"
+
+
+(* TODO: include the log *)
+open FStar.Ghost
+
+val poly1305_blocks_loop:
+  current_log:log_t ->
+  st:poly1305_state ->
+  m:uint8_p ->
+  len:U64.t{U64.v len <= length m} ->
+  r0:limb_44 ->
+  r1:limb_44 ->
+  r2:limb_44 ->
+  s1:limb_44_20{H64 (v s1 = 20 * v r1)} ->
+  s2:limb_44_20{H64 (v s2 = 20 * v r2)} ->
+  h0:limb_45 ->
+  h1:limb_45 ->
+  h2:limb_45 ->
+  Stack log_t
+    (requires (fun h -> live_st h st /\ live h m))
+    (ensures  (fun h0 updated_log h1 -> modifies_1 st.h h0 h1 /\ live_st h1 st
+      /\ (reveal updated_log) ==
+          encode_pad (reveal current_log) (as_seq h0 (Buffer.sub m 0ul (U32 (16ul *^ (Int.Cast.uint64_to_uint32 len)))))
+      /\ sel_elem h1 st.h == poly (reveal updated_log) (sel_elem h0 st.r)))
+let rec poly1305_blocks_loop log st m len r0 r1 r2 s1 s2 h0 h1 h2 =
+  let m0 = ST.get() in
+  let h_0 = h0 in
+  let h_1 = h1 in
+  let h_2 = h2 in
+  if U64 (len <^ 16uL) then (
+    admit();
+    st.h.(0ul) <- h0;
+    st.h.(1ul) <- h1;
+    st.h.(2ul) <- h2;
+    log
+  )
+  else (
+    let t0 = load64_le m in
+    let t1 = load64_le (offset m 8ul) in
+
+    let mask_2_44 = mk_mask 44ul in
+    let mask_2_42 = mk_mask 42ul in
+
+    let open Hacl.UInt64 in
+
+    let t_0 = t0 &^ mask_2_44 in
+    let t_1 = ((t0 >>^ 44ul) |^ (t1 <<^ 20ul)) &^ mask_2_44 in
+    let t_2 = ((t1 >>^ 24ul) &^ mask_2_42) |^ (uint64_to_sint64 1uL <<^ 40ul) in
+
+    assume (eval_3_limbs t_0 t_1 t_2 = pow2 128 + little_endian (sel_word m0 (Buffer.sub m 0ul 16ul)));
+
+    assume (v h0 + v t_0 < pow2 64);
+    let h0 = h0 +^ t_0 in
+    assume (v h1 + v t_1 < pow2 64);
+    let h1 = h1 +^ t_1 in
+    assume (v h2 + v t_2 < pow2 64);
+    let h2 = h2 +^ t_2 in
+
+    assume (eval_3_limbs h0 h1 h2 =
+      pow2 128 + little_endian (sel_word m0 (Buffer.sub m 0ul 16ul))
+      + eval_3_limbs h_0 h_1 h_2);
+
+    let open Hacl.UInt128 in
+    let d0 = h0 *^ r0 in
+    let d  = h1 *^ s2 in
+    assume (v d0 + v d < pow2 128);
+    let d0 = d0 +^ d  in
+    let d  = h2 *^ s1 in
+    assume (v d0 + v d < pow2 128);
+    let d0 = d0 +^ d  in
+
+    let d1 = h0 *^ r1 in
+    let d  = h1 *^ r0 in
+    assume (v d1 + v d < pow2 128);
+    let d1 = d1 +^ d  in
+    let d  = h2 *^ s2 in
+    assume (v d1 + v d < pow2 128);
+    let d1 = d1 +^ d  in
+
+    let d2 = h0 *^ r2 in
+    let d  = h1 *^ r1 in
+    assume (v d2 + v d < pow2 128);
+    let d2 = d2 +^ d  in
+    let d  = h2 *^ r0 in
+    assume (v d2 + v d < pow2 128);
+    let d2 = d2 +^ d  in
+
+    let c  = sint128_to_sint64 (d0 >>^ 44ul) in
+    let h0 = H64 (sint128_to_sint64 d0 &^ mask_2_44) in
+    let d1 = d1 +^ sint64_to_sint128 c in
+
+    let c  = sint128_to_sint64 (d1 >>^ 44ul) in
+    let h1 = H64 (sint128_to_sint64 d1 &^ mask_2_44) in
+    assume (v d2 + H64.v c < pow2 128);
+    let d2 = d2 +^ sint64_to_sint128 c in
+
+    let c  = sint128_to_sint64 (d2 >>^ 42ul) in
+    let h2 = H64 (sint128_to_sint64 d2 &^ mask_2_42) in
+
+    let open Hacl.UInt64 in
+    assume (v c * 5 < pow2 64 /\ v h0 + v c * 5 < pow2 64);
+    let h0 = h0 +^ (c *^ uint64_to_sint64 5uL) in
+    let c  = h0 >>^ 44ul in
+    let h0 = h0 &^ mask_2_44 in
+    assume (v h0 + v c < pow2 64);
+    let h1 = h1 +^ c in
+
+    let len = U64 (len -^ 16uL) in
+    let m   = offset m 16ul in
+    let new_log = elift1 (fun l -> SeqProperties.snoc l (eval_3_limbs h0 h1 h2)) log in
+    poly1305_blocks_loop new_log st m len r0 r1 r2 s1 s2 h0 h1 h2
+  )
+
+
+val poly1305_blocks:
+  log:log_t ->
+  st:poly1305_state ->
+  m:uint8_p ->
+  len:FStar.UInt64.t ->
+  Stack log_t
+    (requires (fun h -> True))
+    (ensures  (fun h0 _ h1 -> True))
+let poly1305_blocks log st m len =
+  let r0 = st.r.(0ul) in
+  let r1 = st.r.(1ul) in
+  let r2 = st.r.(2ul) in
+  let h0 = st.h.(0ul) in
+  let h1 = st.h.(1ul) in
+  let h2 = st.h.(2ul) in
+
+  let five = uint64_to_sint64 5uL in
+  let s1 = H64 (r1 *^ (five <<^ 2ul)) in
+  let s2 = H64 (r2 *^ (five <<^ 2ul)) in
+
+  poly1305_blocks_loop log st m len r0 r1 r2 s1 s2 h0 h1 h2
+
+
+val poly1305_finish:
+  log:log_t ->
+  st:poly1305_state ->
+  mac:uint8_p ->
+  m:uint8_p ->
+  len:U64.t ->
+  key:uint8_p ->
+  Stack log_t
+    (requires (fun _ -> True))
+    (ensures  (fun _ _ _ -> True))
+let poly1305_finish log st mac m len key =
+  push_frame();
+
+  let mask_2_44 = uint64_to_sint64 0xfffffffffffuL in
+  let mask_2_42 = uint64_to_sint64 0x3ffffffffffuL in
+
+  let rem = U64 (len &^ 0xfuL) in
+
+  let h0 = st.h.(0ul) in
+  let h1 = st.h.(1ul) in
+  let h2 = st.h.(2ul) in
+  let r0 = st.r.(0ul) in
+  let r1 = st.r.(1ul) in
+  let r2 = st.r.(2ul) in
+  let five = uint64_to_sint64 5uL in
+  let s1 = H64 (r1 *^ (five <<^ 2ul)) in
+  let s2 = H64 (r2 *^ (five <<^ 2ul)) in
+
+    if U64 (rem =^ 0uL) then ()
+    else (
+      let zero = uint8_to_sint8 0uy in
+      let block = create zero 16ul in
+      let i = FStar.Int.Cast.uint64_to_uint32 rem in
+      blit m (FStar.Int.Cast.uint64_to_uint32 (U64 (len -^ rem))) block 0ul i;
+      block.(i) <- uint8_to_sint8 1uy;
+
+      let t0 = load64_le block in
+      let t1 = load64_le (offset block 8ul) in
+
+      let open Hacl.UInt64 in
+
+      let h0 = h0 +^ (t0 &^ mask_2_44) in
+      let h1 = h1 +^ (((t0 >>^ 44ul) |^ (t1 <<^ 20ul)) &^ mask_2_44) in
+      let h2 = h2 +^ ((t1 >>^ 24ul) &^ mask_2_42) in
+
+      let open Hacl.UInt128 in
+
+      let d0 = h0 *^ r0 in
+      let d  = h1 *^ s2 in
+      let d0 = d0 +^ d  in
+      let d  = h2 *^ s1 in
+      let d0 = d0 +^ d  in
+
+      let d1 = h0 *^ r1 in
+      let d  = h1 *^ r0 in
+      let d1 = d1 +^ d  in
+      let d  = h2 *^ s2 in
+      let d1 = d1 +^ d  in
+
+      let d2 = h0 *^ r2 in
+      let d  = h1 *^ r1 in
+      let d2 = d2 +^ d  in
+      let d  = h2 *^ r0 in
+      let d2 = d2 +^ d  in
+
+      let c  = sint128_to_sint64 (d0 >>^ 44ul) in
+      let h0 = H64 (sint128_to_sint64 d0 &^ mask_2_44) in
+      let d1 = d1 +^ sint64_to_sint128 c in
+
+      let c  = sint128_to_sint64 (d1 >>^ 44ul) in
+      let h1 = H64 (sint128_to_sint64 d1 &^ mask_2_44) in
+      let d2 = d2 +^ sint64_to_sint128 c in
+
+      let c  = sint128_to_sint64 (d2 >>^ 42ul) in
+      let h2 = H64 (sint128_to_sint64 d2 &^ mask_2_42) in
+
+      let open Hacl.UInt64 in
+      let h0 = h0 +^ (c *^ uint64_to_sint64 5uL) in
+      let c  = h0 >>^ 44ul in
+      let h0 = h0 &^ mask_2_44 in
+      let h1 = h1 +^ c in
+      st.h.(0ul) <- h0;
+      st.h.(1ul) <- h1;
+      st.h.(2ul) <- h2
+    );
+
+  let h0 = st.h.(0ul) in
+  let h1 = st.h.(1ul) in
+  let h2 = st.h.(2ul) in
+
+  let open Hacl.UInt64 in
+
+  let c  = h1 >>^ 44ul in
+  let h1 = h1 &^ mask_2_44 in
+  let h2 = h2 +^ c in
+  let c  = h2 >>^ 42ul in
+  let h2 = h2 &^ mask_2_42 in
+  let h0 = h0 +^ (c *^ uint64_to_sint64 5uL) in
+  let c  = h0 >>^ 44ul in
+  let h0 = h0 &^ mask_2_44 in
+  let h1 = h1 +^ c in
+  let c  = h1 >>^ 44ul in
+  let h1 = h1 &^ mask_2_44 in
+  let h2 = h2 +^ c in
+  let c  = h2 >>^ 42ul in
+  let h2 = h2 &^ mask_2_42 in
+  let h0 = h0 +^ (c *^ uint64_to_sint64 5uL) in
+  let c  = h0 >>^ 44ul in
+  let h0 = h0 &^ mask_2_44 in
+  let h1 = h1 +^ c in
+
+  let mask = (eq_mask h0 mask_2_44)
+             &^ (eq_mask h1 mask_2_44)
+             &^ (gte_mask h2 (uint64_to_sint64 0x3fffffffffbuL)) in
+  let h0 = h0 &^ lognot mask in
+  let h1 = h1 &^ lognot mask in
+  let h2 = h2 -^ ((uint64_to_sint64 0x3fffffffffbuL) &^ mask) in
+
+  let t0 = load64_le (offset key 16ul) in
+  let t1 = load64_le (offset key 24ul) in
+
+  let h0 = h0 +^ (t0 &^ mask_2_44) in
+  let c  = h0 >>^ 44ul in
+  let h0 = h0 &^ mask_2_44 in
+  let h1 = h1 +^ (((t0 >>^ 44ul) |^ (t1 <<^ 20ul)) &^ mask_2_44) +^ c in
+  let c  = h1 >>^ 44ul in
+  let h1 = h1 &^ mask_2_44 in
+  let h2 = h2 +^ ((t1 >>^ 24ul) &^ mask_2_42) +^ c in
+  let h2 = h2 &^ mask_2_42 in
+
+  let h0 = h0 |^ (h1 <<^ 44ul) in
+  let h1 = (h1 >>^ 20ul) |^ (h2 <<^ 24ul) in
+
+  store64_le mac h0;
+  store64_le (offset mac 8ul) h1;
+  pop_frame();
+  log // TODO
+
+val crypto_onetimeauth:
+  output:uint8_p ->
+  input:uint8_p ->
+  len:U64.t ->
+  k:uint8_p ->
+  Stack unit
+    (requires (fun _ -> True))
+    (ensures  (fun _ _ _ -> True))
+let crypto_onetimeauth output input len k =
+  push_frame();
+  let zero = uint64_to_sint64 0uL in
+  let r = create zero 3ul in
+  let h = create zero 3ul in
+  let st = {r = r; h = h} in
+  let init_log = poly1305_init st k in
+  let partial_log = poly1305_blocks init_log st input len in
+  let final_log = poly1305_finish partial_log st output input len k in
+  pop_frame()
